src/NaturalDeductionToLatex.v
@@ -13,43 +13,14 @@ Section ToLatex.
 
   Context {Judgment : Type}.
   Context {Rule     : forall (hypotheses:Tree ??Judgment)(conclusion:Tree ??Judgment), Type}.
-
-  (* the "user" must supply functions for latexifying judgments and rules *)
-  Context (judgment2latex : Judgment -> string).
-  Context (rule2latex     : forall h c, Rule h c -> string).
+  Context {JudgmentToLatexMath : ToLatexMath Judgment}.
+  Context {RuleToLatexMath     : forall h c, ToLatexMath (Rule h c)}.
   
   Open Scope string_scope.
-  Notation "a +++ b" := (append a b) (at level 100).
-  Section TreeToLatex.
-    Context (emptyleaf:string).
-    Context {T:Type}.
-    Context (leaf:T -> string).
-    Fixpoint tree2latex' (j:Tree ??T) : string :=
-      match j with
-        | T_Leaf   None      => emptyleaf
-        | T_Leaf   (Some j') => leaf j'
-        | T_Branch b1 b2     => "\left["+++tree2latex' b1+++
-                                "\text{\tt{,}}"+++
-                                tree2latex' b2+++"\right]"
-      end.
-    Definition tree2latex (j:Tree ??T) : string :=
-      match j with
-        | T_Leaf   None      => emptyleaf
-        | T_Leaf   (Some j') => leaf j'
-        | T_Branch b1 b2     => tree2latex' b1+++
-                                "\text{\tt{,}}"+++
-                                tree2latex' b2
-      end.
-    Fixpoint list2latex (sep:string)(l:list T) : string :=
-      match l with
-        | nil      => emptyleaf
-        | (a::nil) => leaf a
-        | (a::b)   => (leaf a)+++sep+++(list2latex sep b)
-      end.
-  End TreeToLatex.
 
-  Definition judgments2latex (j:Tree ??Judgment) := 
-    list2latex " " judgment2latex " \\ " (leaves j).
+  Definition judgments2latex (j:Tree ??Judgment) := treeToLatexMath (mapOptionTree toLatexMath j).
+
+  Definition eolL : LatexMath := rawLatexMath eol.
 
   (* invariant: each proof shall emit its hypotheses visibly, except nd_id0 *)
   Section SCND_toLatex.
@@ -57,46 +28,62 @@ Section ToLatex.
     (* indicates which rules should be hidden (omitted) from the rendered proof; useful for structural operations *)
     Context (hideRule : forall h c (r:Rule h c), bool).
 
-    Fixpoint SCND_toLatex {h}{c}(pns:SCND h c) : string :=
+    Fixpoint SCND_toLatexMath {h}{c}(pns:SCND(Rule:=Rule) h c) : LatexMath :=
       match pns with
-        | scnd_leaf   ht c pn            => SCND_toLatex pn
-        | scnd_branch ht c1 c2 pns1 pns2 => SCND_toLatex pns1 +++ " \hspace{1cm} " +++ SCND_toLatex pns2
-        | scnd_weak     c                => ""
-        | scnd_comp ht ct c pns rule => if hideRule _ _ rule
-                                      then SCND_toLatex pns
-                                      else "\trfrac["+++rule2latex _ _ rule +++ "]{" +++ eol +++
-                                             SCND_toLatex pns +++ "}{" +++ eol +++
-                                             judgment2latex c +++ "}" +++ eol
+        | scnd_leaf   ht c pn            => SCND_toLatexMath pn
+        | scnd_branch ht c1 c2 pns1 pns2 => SCND_toLatexMath pns1 +++ rawLatexMath " \hspace{1cm} " +++ SCND_toLatexMath pns2
+        | scnd_weak     c                => rawLatexMath ""
+        | scnd_comp ht ct c pns rule     => if hideRule _ _ rule
+                                            then SCND_toLatexMath pns
+                                            else rawLatexMath "\trfrac["+++ toLatexMath rule +++ rawLatexMath "]{" +++ eolL +++
+                                              SCND_toLatexMath pns +++ rawLatexMath "}{" +++ eolL +++
+                                              toLatexMath c +++ rawLatexMath "}" +++ eolL
       end.
   End SCND_toLatex.
 
-  (* this is a work-in-progress; please use SCND_toLatex for now *)
-  Fixpoint nd_toLatex {h}{c}(nd:@ND _ Rule h c)(indent:string) :=
+  (* this is a work-in-progress; please use SCND_toLatexMath for now *)
+  Fixpoint nd_toLatexMath {h}{c}(nd:@ND _ Rule h c)(indent:string) :=
     match nd with
-      | nd_id0                      => indent +++ "% nd_id0 " +++ eol
-      | nd_id1  h'                  => indent +++ "% nd_id1 "+++ judgments2latex h +++ eol
-      | nd_weak h'                  => indent +++ "\inferrule*[Left=ndWeak]{" +++ judgment2latex h' +++ "}{ }" +++ eol
-      | nd_copy h'                  => indent +++ "\inferrule*[Left=ndCopy]{"+++judgments2latex h+++
-                                                         "}{"+++judgments2latex c+++"}" +++ eol
-      | nd_prod h1 h2 c1 c2 pf1 pf2 => indent +++ "% prod " +++ eol +++
-                                       indent +++ "\begin{array}{c c}" +++ eol +++
-                                       (nd_toLatex pf1 ("  "+++indent)) +++
-                                       indent +++ " & " +++ eol +++
-                                       (nd_toLatex pf2 ("  "+++indent)) +++
-                                       indent +++ "\end{array}"
-      | nd_comp h  m     c  pf1 pf2 => indent +++ "% comp " +++ eol +++
-                                       indent +++ "\begin{array}{c}" +++ eol +++
-                                       (nd_toLatex pf1 ("  "+++indent)) +++
-                                       indent +++ " \\ " +++ eol +++
-                                       (nd_toLatex pf2 ("  "+++indent)) +++
-                                       indent +++ "\end{array}"
-      | nd_cancell a                => indent +++ "% nd-cancell " +++ (judgments2latex a) +++ eol
-      | nd_cancelr a                => indent +++ "% nd-cancelr " +++ (judgments2latex a) +++ eol
-      | nd_llecnac a                => indent +++ "% nd-llecnac " +++ (judgments2latex a) +++ eol
-      | nd_rlecnac a                => indent +++ "% nd-rlecnac " +++ (judgments2latex a) +++ eol
-      | nd_assoc   a b c            => ""
-      | nd_cossa   a b c            => ""
-      | nd_rule    h c r            => rule2latex h c r
+      | nd_id0                      => rawLatexMath indent +++
+                                       rawLatexMath "% nd_id0 " +++ eolL
+      | nd_id1  h'                  => rawLatexMath indent +++
+                                       rawLatexMath "% nd_id1 "+++ judgments2latex h +++ eolL
+      | nd_weak h'                  => rawLatexMath indent +++
+                                       rawLatexMath "\inferrule*[Left=ndWeak]{" +++ toLatexMath h' +++ rawLatexMath "}{ }" +++ eolL
+      | nd_copy h'                  => rawLatexMath indent +++
+                                       rawLatexMath "\inferrule*[Left=ndCopy]{"+++judgments2latex h+++
+                                                         rawLatexMath "}{"+++judgments2latex c+++rawLatexMath "}" +++ eolL
+      | nd_prod h1 h2 c1 c2 pf1 pf2 => rawLatexMath indent +++
+                                       rawLatexMath "% prod " +++ eolL +++
+                                       rawLatexMath indent +++
+                                       rawLatexMath "\begin{array}{c c}" +++ eolL +++
+                                       (nd_toLatexMath pf1 ("  "+++indent)) +++
+                                       rawLatexMath indent +++
+                                       rawLatexMath " & " +++ eolL +++
+                                       (nd_toLatexMath pf2 ("  "+++indent)) +++
+                                       rawLatexMath indent +++
+                                       rawLatexMath "\end{array}"
+      | nd_comp h  m     c  pf1 pf2 => rawLatexMath indent +++
+                                       rawLatexMath "% comp " +++ eolL +++
+                                       rawLatexMath indent +++
+                                       rawLatexMath "\begin{array}{c}" +++ eolL +++
+                                       (nd_toLatexMath pf1 ("  "+++indent)) +++
+                                       rawLatexMath indent +++
+                                       rawLatexMath " \\ " +++ eolL +++
+                                       (nd_toLatexMath pf2 ("  "+++indent)) +++
+                                       rawLatexMath indent +++
+                                       rawLatexMath "\end{array}"
+      | nd_cancell a                => rawLatexMath indent +++
+                                       rawLatexMath "% nd-cancell " +++ (judgments2latex a) +++ eolL
+      | nd_cancelr a                => rawLatexMath indent +++
+                                       rawLatexMath "% nd-cancelr " +++ (judgments2latex a) +++ eolL
+      | nd_llecnac a                => rawLatexMath indent +++
+                                       rawLatexMath "% nd-llecnac " +++ (judgments2latex a) +++ eolL
+      | nd_rlecnac a                => rawLatexMath indent +++
+                                       rawLatexMath "% nd-rlecnac " +++ (judgments2latex a) +++ eolL
+      | nd_assoc   a b c            => rawLatexMath ""
+      | nd_cossa   a b c            => rawLatexMath ""
+      | nd_rule    h c r            => toLatexMath r
     end.
 
 End ToLatex.
